src/tls/ConnInvariant.fst
@@ -111,7 +111,7 @@ type c_t  = MM.map' random r_conn
 
 //w is registered with c, in state h
 let registered (i:id{StAE.is_stream i}) (w:StreamAE.writer i) (c:connection) (h:HH.t) =
-  (exists e. SeqProperties.mem e  (epochs c h) /\               //one of c's epochs, e
+  (exists e. (epochs c h) `SeqP.contains` e  /\               //one of c's epochs, e
       (let i' = Epochs.epoch_id e in   //has an id corresponding to i
         i=i' /\ StAE.stream_state #i e.w == w))               //and holds w as as its writer
   /\ MonSeq.i_contains (MkEpochs.es c.hs.log) h                         //technical: the heap contains c's handshake log
@@ -255,17 +255,10 @@ let writer_region_within_connection
 	    (ensures (HH.includes (C.region c) (StreamAE.State.region w)))
     = reveal_epoch_region_inv_all ()
 
-//A wrapper around a Sequence lemma ... should move it
-let lemma_mem_snoc (#a:eqtype) (s:FStar.Seq.seq a) (x:a)
-  : Lemma (ensures (forall y.{:pattern (SeqProperties.mem y (SeqProperties.snoc s x))}
-      SeqProperties.mem y (SeqProperties.snoc s x) <==> SeqProperties.mem y s \/ x=y))
-  = SeqProperties.lemma_mem_snoc s x
-
-
 (* Case 2:
      Adding a new epoch to a connection c, with a fresh index (hdId i) for c
       -- we found a writer w at (ms i), pre-allocated (we're second) or not (we're first)
-      -- we need to show that the (exists e. SeqProperties.mem ...) is false (because of the fresh index for c)
+      -- we need to show that the (exists e. SeqProperties.contains ...) is false (because of the fresh index for c)
       -- so, we're in the "not yet used" case ... so, the epoch's writer is in its initial state and we can return it (our goal is to return a fresh epoch)
 *)
 val register_writer_in_epoch_ok: h0:HyperHeap.t -> h1:HyperHeap.t -> i:AE.id{authId i}
@@ -286,7 +279,7 @@ val register_writer_in_epoch_ok: h0:HyperHeap.t -> h1:HyperHeap.t -> i:AE.id{aut
               N.registered (nonce_of_id i) (HH.parent (StreamAE.State.region w)) /\  //the writer's parent region is registered in the nonce table
 	      HH.disjoint (HH.parent (StreamAE.State.region w)) tls_region /\          //technical: ... needed just for well-formedness of the rest of the formula
 	      MR.witnessed (MR.rid_exists (StreamAE.State.region w)) /\                //technical: ... needed just for well-formedness of the rest of the formula
-	      (forall e. SeqProperties.mem e epochs ==> Epochs.epoch_id e <> i) /\            //i is fresh for c
+	      (forall e. epochs `SeqP.contains` e ==> Epochs.epoch_id e <> i) /\            //i is fresh for c
  	      MM.sel mstab i == Some w /\ //we found the writer in the ms_tab
 	      MM.sel ctab (nonce_of_id i) == Some c /\ //we found the connection in the conn_table
       	      HH.modifies_one (HS.region c.hs) h0 h1 /\ //we just modified this connection's handshake region
@@ -309,7 +302,7 @@ let register_writer_in_epoch_ok h0 h1 i c e =
       let old_hs_log = epochs c h0 in
       let wi = StAE.stream_state #i (Epoch.w e) in //the epoch writer
       let nonce = nonce_of_id i in
-      lemma_mem_snoc old_hs_log e; //this lemma shows that everything that was registered to c remains registered to it
+      SeqP.contains_snoc old_hs_log e; //this lemma shows that everything that was registered to c remains registered to it
       assert (old_ms == new_ms);
       assert (old_conn == new_conn);
       cut (is_Some (MM.sel old_conn nonce)); //this cut is useful for triggering the pairwise_disjointness quantifier
